NumLean/Data/TensorIndex.lean
@@ -1,5 +1,6 @@
 import NumLean.Data.TensorIndex.Basic
-import NumLean.Data.TensorIndex.NatFinTIndex
+import NumLean.Data.TensorIndex.IntFinTIndex
+import NumLean.Data.TensorIndex.FinTIndexFold
 import NumLean.Data.TensorIndex.FinTIndexIterator
 import NumLean.Data.TensorIndex.Compatibility
 import NumLean.Data.TensorIndex.Layout
